preuve insert générique

projet.v
@@ -40,12 +40,13 @@ match l with
 | z::l' => insert z (insertion_sort l')
 end.
 
-(*
-Inductive sorted
-Hint Resolve sorted0 sorted1 sorted2 : sort.
-Lemma sort_2357
-Theorem sorted_inv
-*)
+Inductive sorted : list T -> Prop :=
+  | sorted0 : sorted nil
+  | sorted1 : forall t:T, sorted (t :: nil)
+  | sorted2 :
+      forall (t1 t2:T) (l:list T),
+        (leb t1 t2) = true ->
+        sorted (t2 :: l) -> sorted (t1 :: t2 :: l).
 
 Fixpoint nb_occ (z:T) (l:list T) {struct l} : nat :=
   match l with
@@ -59,23 +60,73 @@ Fixpoint nb_occ (z:T) (l:list T) {struct l} : nat :=
 Definition equiv (l l':list T) := 
     forall z:T, nb_occ z l = nb_occ z l'.
 
-(*
-Definition equiv
-Lemma equiv_refl
-Lemma equiv_sym
-Lemma equiv_trans
-Lemma equiv_cons
-Lemma equiv_perm
+Hint Resolve sorted0 sorted1 sorted2 : sort.
+Theorem sorted_inv :
+ forall (z:T) (l:list T), sorted (z :: l) -> sorted l.
+Proof.
+ intros z l H.
+ inversion H; auto with sort.
+Qed.
+
+Lemma equiv_refl : forall l:list T, equiv l l.
+Proof.
+ unfold equiv; trivial.
+Qed.
+
+Lemma equiv_sym : forall l l':list T, equiv l l' -> equiv l' l.
+Proof.
+  unfold equiv; auto.
+Qed.
+
+Lemma equiv_trans :
+ forall l l' l'':list T, equiv l l' -> 
+                         equiv l' l'' -> 
+                         equiv l l''.
+Proof.
+ intros l l' l'' H H0 z.
+ eapply trans_eq; eauto.
+Qed.
+
+Lemma equiv_cons :
+ forall (t:T) (l l':list T), equiv l l' -> 
+                             equiv (t :: l) (t :: l').
+Proof.
+ intros t l l' H t'.
+ simpl; case_eq  (eqb t' t); auto. 
+Qed.
+
+Lemma equiv_perm :
+ forall (a b:T) (l l':list T),
+   equiv l l' -> 
+   equiv (a :: b :: l) (b :: a :: l').
+Proof.
+ intros a b l l' H t; simpl.
+ case_eq (eqb t a); case_eq (eqb t b); 
+  simpl; case (H t); auto.
+Qed.
+
 Hint Resolve equiv_cons equiv_refl equiv_perm : sort.
-...
-*)
+
 End poly.
 
 About insert.
 Open Scope Z_scope.
 
+Hint Resolve sorted0 sorted1 sorted2 : sort.
+Lemma sort_2357 :
+ sorted Z Z.leb (2 :: 3 :: 5 :: 7 :: nil).
+Proof.
+ auto with sort zarith.
+Qed.
+
 Section Tests.
 Compute insert Z Z.leb 4 (2 :: 5 :: nil).
 Compute insertion_sort Z Z.leb (4::9::7::9::12::3::nil).
 Eval compute in (nb_occ Z Z.eqb 3 (3 :: 7 :: 3 :: nil)).
+
+Compute insert Z Z.geb 4 (5 :: 2 :: nil).
+Compute insertion_sort Z Z.geb (4::9::7::9::12::3::nil).
+
+Require Import Ascii.
+
 End Tests.
